lib: refactor time_methods and test cases

lib/Time_Methods_Cmd.thy
@@ -1,5 +1,4 @@
 (*
- *
  * Copyright 2018, Data61, CSIRO
  *
  * This software may be distributed and modified according to the terms of
@@ -10,122 +9,98 @@
  *)
 
 theory Time_Methods_Cmd imports
-  Eisbach_Methods
+  Main
 begin
 
-text \<open>
-  Utility that runs several methods on the same proof goal, printing the
-  running time of each one.
+(* See Time_Methods_Cmd_Test for documentation *)
 
-  Usage:
-
-    apply (time_methods [(no_check)]
-        [name1:] \<open>method1\<close>
-        [name2:] \<open>method2\<close>
-        ...)
-
-  See the examples at the end of this theory.
-\<close>
-
-ML {*
-*}
-method_setup time_methods =
- \<open>
-let
-  (* Work around Isabelle running every apply method on an empty proof state *)
-  fun skip_dummy_state tactic = fn st =>
+ML \<open>
+structure Time_Methods = struct
+  (* Work around Isabelle running every apply method on a dummy proof state *)
+  fun skip_dummy_state (method: Method.method) : Method.method =
+    fn facts => fn (ctxt, st) =>
       case Thm.prop_of st of
           Const ("Pure.prop", _) $ (Const ("Pure.term", _) $ Const ("Pure.dummy_pattern", _)) =>
-            Seq.succeed st
-        | _ => tactic st;
-in
-  Scan.lift (Scan.optional (Args.parens (Parse.reserved "no_check") >> K true) false) --
-  Scan.repeat1 (Scan.option (Scan.lift (Parse.liberal_name --| Parse.$$$ ":")) -- Method.text_closure) >>
-  (fn (no_check, maybe_named_methods) => fn ctxt => fn facts => let
-        val named_methods = tag_list 1 maybe_named_methods
-                |> map (fn (i, (maybe_name, method)) =>
-                        case maybe_name of SOME name => (name, method)
-                                         | NONE => ("[method " ^ string_of_int i ^ "]", method))
-        fun tac st = let
-            fun run name method =
-                  Timing.timing (fn () => case method_evaluate method ctxt facts st |> Seq.pull of
-                        NONE => (NONE, Seq.empty)
-                      | SOME (st', sts') => (SOME st', Seq.cons st' sts')) ()
-            val results = named_methods |> map (fn (name, method) =>
-                  let val (time, (st', results)) = run name method
-                      val _ = warning (name ^ ": " ^ Timing.message time)
-                  in {name = name, state = st', results = results} end)
-            val canonical_result = hd results
-            val other_results = tl results
-          in
-            if no_check then #results canonical_result else
-            case other_results |> filter (fn result =>
-                      Option.map Thm.full_prop_of (#state result) <>
-                      Option.map Thm.full_prop_of (#state canonical_result)) of
-                [] => #results canonical_result
-              | (bad::_) => raise THM ("methods \"" ^ #name canonical_result ^
-                                       "\" and \"" ^ #name bad ^ "\" have different results",
-                                       1, the_list (#state canonical_result) @ the_list (#state bad))
-          end
-     in SIMPLE_METHOD (skip_dummy_state tac) [] end)
+            Seq.succeed (Seq.Result (ctxt, st))
+        | _ => method facts (ctxt, st);
+
+  (* ML interface. Takes a list of (possibly-named) methods, then calls the supplied
+   * callback with the method index (starting from 1), supplied name and timing.
+   * Also returns the list of timings at the end. *)
+  fun time_methods
+        (no_check: bool)
+        (callback: (int * string option -> Timing.timing -> unit))
+        (maybe_named_methods: (string option * Method.method) list)
+        (* like Method.method but also returns timing list *)
+        : thm list -> context_state -> (Timing.timing list * context_state Seq.result Seq.seq)
+    = fn facts => fn (ctxt, st) => let
+        fun run method =
+              Timing.timing (fn () =>
+                case method facts (ctxt, st) |> Seq.pull of
+                  (* Peek at first result, then put it back *)
+                    NONE => (NONE, Seq.empty)
+                  | SOME (r as Seq.Result (_, st'), rs) => (SOME st', Seq.cons r rs)
+                  | SOME (r as Seq.Error _, rs) => (NONE, Seq.cons r rs)
+              ) ()
+
+        val results = tag_list 1 maybe_named_methods
+              |> map (fn (idx1, (maybe_name, method)) =>
+                  let val (time, (st', results)) = run method
+                      val _ = callback (idx1, maybe_name) time
+                      val name = Option.getOpt (maybe_name, "[method " ^ string_of_int idx1 ^ "]")
+                  in {name = name, state = st', results = results, time = time} end)
+
+        val canonical_result = hd results
+        val other_results = tl results
+        val return_val = (map #time results, #results canonical_result)
+        fun show_state NONE = @{thm FalseE[where P="METHOD_FAILED"]}
+          | show_state (SOME st) = st
+      in
+        if no_check then return_val else
+        (* Compare the proof states that we peeked at *)
+        case other_results
+              |> filter (fn result =>
+                    (* It's tempting to use aconv, etc., here instead of op<>, but
+                     * minute differences such as bound names in Pure.all can
+                     * break a proof script later on. *)
+                    Option.map Thm.full_prop_of (#state result) <>
+                    Option.map Thm.full_prop_of (#state canonical_result)) of
+            [] => return_val
+          | (bad_result::_) =>
+              raise THM ("methods \"" ^ #name canonical_result ^
+                         "\" and \"" ^ #name bad_result ^ "\" have different results",
+                         1, map (show_state o #state) [canonical_result, bad_result])
+      end
 end
 \<close>
 
-text \<open>Examples\<close>
-experiment begin
-  lemma
-    "a = b \<Longrightarrow> b = c \<Longrightarrow> a = c"
-    apply (time_methods
-            \<open>rule back_subst[where P="op= a"], assumption+\<close>
-            \<open>rule trans, assumption+\<close>)
-    done
-
-  lemma
-    "a = b \<Longrightarrow> b = c \<Longrightarrow> a = c"
-    apply (time_methods (no_check)
-            \<open>rule back_subst[where P="op= a"]\<close>
-            \<open>rule trans\<close>)
-     text \<open>no_check prevents failing even though the method results differ\<close>
-     apply assumption+
-    done
-
-  text \<open>
-    Fast and slow list reversals
-  \<close>
-  lemma list_eval_rev_append:
-    "rev xs = rev xs @ []"
-    "rev [] @ ys = ys"
-    "rev (x # xs) @ ys = rev xs @ (x # ys)"
-    by auto
-
-  lemma "rev [10..90] = map (op- 100) [10..90]"
-        "rev [10..290] = map (op- 300) [10..290]"
-    text \<open>evaluate everything but @{term rev}\<close>
-    apply (all \<open>match conclusion in "rev x = y" for x y \<Rightarrow>
-                  \<open>rule subst[where t = x], simp\<close>\<close>)
-    apply (all \<open>match conclusion in "rev x = y" for x y \<Rightarrow>
-                  \<open>rule subst[where t = y], simp\<close>\<close>)
-
-    text \<open>evaluate @{term rev}\<close>
-    apply (time_methods
-            simp: \<open>simp\<close>
-            slow: \<open>simp only: rev.simps append.simps\<close>
-            fast: \<open>subst list_eval_rev_append(1), simp only: list_eval_rev_append(2-3)\<close>
-          )
-    apply (time_methods
-            simp: \<open>simp\<close>
-            slow: \<open>simp only: rev.simps append.simps\<close>
-            fast: \<open>subst list_eval_rev_append(1), simp only: list_eval_rev_append(2-3)\<close>
-          )
-    done
-
-
-  text \<open>Other tests\<close>
-
-  lemma "A"
-    -- "simp should fail and time_methods should propagate the failure"
-    apply (fails \<open>time_methods \<open>simp\<close>\<close>)
-    oops
+method_setup time_methods = \<open>
+let
+  val parse_no_check = Scan.lift (Scan.optional (Args.parens (Parse.reserved "no_check") >> K true) false)
+  val parse_maybe_name = Scan.option (Scan.lift (Parse.liberal_name --| Parse.$$$ ":"))
+  fun auto_name (idx1, maybe_name) =
+        Option.getOpt (maybe_name, "[method " ^ string_of_int idx1 ^ "]")
+in
+  parse_no_check --
+  Scan.repeat1 (parse_maybe_name -- Method.text_closure) >>
+  (fn (no_check, maybe_named_methods_text) => fn ctxt =>
+      let
+        val max_length = tag_list 1 (map fst maybe_named_methods_text)
+                         |> map (String.size o auto_name)
+                         |> (fn ls => fold (curry Int.max) ls 0)
+        fun pad_name s =
+           let val pad_length = max_length + String.size ": " - String.size s
+           in s ^ replicate_string pad_length " " end
+        fun timing_callback id time = warning (pad_name (auto_name id ^ ": ") ^ Timing.message time)
+        val maybe_named_methods = maybe_named_methods_text
+              |> map (apsnd (fn method_text => Method.evaluate method_text ctxt))
+        val timed_method = Time_Methods.time_methods no_check timing_callback maybe_named_methods
+        fun method_discard_times facts st = snd (timed_method facts st)
+      in
+        method_discard_times
+        |> Time_Methods.skip_dummy_state
+      end)
 end
+\<close>
 
 end
